Show that default state satisfies the relation

examples/tutorial/2-lift/tutorial_liftScript.sml
@@ -101,6 +101,245 @@ val bool2w_and = prove(``!a b. ((bool2w a) && (bool2w b)) = (bool2w (a /\ b))``,
 val imm_eq_to_val_eq = prove(``!a b . ((BVal_Imm(Imm1 a)) = (BVal_Imm(Imm1 b))) = (a = b)``,
     REPEAT STRIP_TAC >> EVAL_TAC);
 
+
+
+val arm8_wf_varset_def = Define `
+arm8_wf_varset vset =
+  (vset = {
+  (BVar "ProcState_C" (BType_Imm Bit1));
+  (BVar "tmp_ProcState_C" (BType_Imm Bit1));
+  (BVar "ProcState_N" (BType_Imm Bit1));
+  (BVar "tmp_ProcState_N" (BType_Imm Bit1));
+  (BVar "ProcState_V" (BType_Imm Bit1));
+  (BVar "tmp_ProcState_V" (BType_Imm Bit1));
+  (BVar "ProcState_Z" (BType_Imm Bit1));
+  (BVar "tmp_ProcState_Z" (BType_Imm Bit1));
+  (BVar "R0" (BType_Imm Bit64));
+  (BVar "tmp_R0" (BType_Imm Bit64));
+  (BVar "R1" (BType_Imm Bit64));
+  (BVar "tmp_R1" (BType_Imm Bit64));
+  (BVar "R2" (BType_Imm Bit64));
+  (BVar "tmp_R2" (BType_Imm Bit64));
+  (BVar "R3" (BType_Imm Bit64));
+  (BVar "tmp_R3" (BType_Imm Bit64));
+  (BVar "R4" (BType_Imm Bit64));
+  (BVar "tmp_R4" (BType_Imm Bit64));
+  (BVar "R5" (BType_Imm Bit64));
+  (BVar "tmp_R5" (BType_Imm Bit64));
+  (BVar "R6" (BType_Imm Bit64));
+  (BVar "tmp_R6" (BType_Imm Bit64));
+  (BVar "R7" (BType_Imm Bit64));
+  (BVar "tmp_R7" (BType_Imm Bit64));
+  (BVar "R8" (BType_Imm Bit64));
+  (BVar "tmp_R8" (BType_Imm Bit64));
+  (BVar "R9" (BType_Imm Bit64));
+  (BVar "tmp_R9" (BType_Imm Bit64));
+  (BVar "R10" (BType_Imm Bit64));
+  (BVar "tmp_R10" (BType_Imm Bit64));
+  (BVar "R11" (BType_Imm Bit64));
+  (BVar "tmp_R11" (BType_Imm Bit64));
+  (BVar "R12" (BType_Imm Bit64));
+  (BVar "tmp_R12" (BType_Imm Bit64));
+  (BVar "R13" (BType_Imm Bit64));
+  (BVar "tmp_R13" (BType_Imm Bit64));
+  (BVar "R14" (BType_Imm Bit64));
+  (BVar "tmp_R14" (BType_Imm Bit64));
+  (BVar "R15" (BType_Imm Bit64));
+  (BVar "tmp_R15" (BType_Imm Bit64));
+  (BVar "R16" (BType_Imm Bit64));
+  (BVar "tmp_R16" (BType_Imm Bit64));
+  (BVar "R17" (BType_Imm Bit64));
+  (BVar "tmp_R17" (BType_Imm Bit64));
+  (BVar "R18" (BType_Imm Bit64));
+  (BVar "tmp_R18" (BType_Imm Bit64));
+  (BVar "R19" (BType_Imm Bit64));
+  (BVar "tmp_R19" (BType_Imm Bit64));
+  (BVar "R20" (BType_Imm Bit64));
+  (BVar "tmp_R20" (BType_Imm Bit64));
+  (BVar "R21" (BType_Imm Bit64));
+  (BVar "tmp_R21" (BType_Imm Bit64));
+  (BVar "R22" (BType_Imm Bit64));
+  (BVar "tmp_R22" (BType_Imm Bit64));
+  (BVar "R23" (BType_Imm Bit64));
+  (BVar "tmp_R23" (BType_Imm Bit64));
+  (BVar "R24" (BType_Imm Bit64));
+  (BVar "tmp_R24" (BType_Imm Bit64));
+  (BVar "R25" (BType_Imm Bit64));
+  (BVar "tmp_R25" (BType_Imm Bit64));
+  (BVar "R26" (BType_Imm Bit64));
+  (BVar "tmp_R26" (BType_Imm Bit64));
+  (BVar "R27" (BType_Imm Bit64));
+  (BVar "tmp_R27" (BType_Imm Bit64));
+  (BVar "R28" (BType_Imm Bit64));
+  (BVar "tmp_R28" (BType_Imm Bit64));
+  (BVar "R29" (BType_Imm Bit64));
+  (BVar "tmp_R29" (BType_Imm Bit64));
+  (BVar "R30" (BType_Imm Bit64));
+  (BVar "tmp_R30" (BType_Imm Bit64));
+  (BVar "R31" (BType_Imm Bit64));
+  (BVar "tmp_R31" (BType_Imm Bit64));
+  (BVar "SP_EL0" (BType_Imm Bit64));
+  (BVar "tmp_SP_EL0" (BType_Imm Bit64));
+  (BVar "SP_EL1" (BType_Imm Bit64));
+  (BVar "tmp_SP_EL1" (BType_Imm Bit64));
+  (BVar "SP_EL2" (BType_Imm Bit64));
+  (BVar "tmp_SP_EL2" (BType_Imm Bit64));
+  (BVar "SP_EL3" (BType_Imm Bit64));
+  (BVar "tmp_SP_EL3" (BType_Imm Bit64));
+  (BVar "MEM" (BType_Mem Bit64 Bit8));
+  (BVar "tmp_MEM" (BType_Mem Bit64 Bit8));
+  (BVar "tmp_PC" (BType_Imm Bit64));
+  (BVar "tmp_COND" (BType_Imm Bit1))
+})`;
+  
+
+
+val default_arm8_bir_state_def = Define `default_arm8_bir_state ms =
+ <|bst_pc :=  bir_block_pc (BL_Address (Imm64 ms.PC)); 
+ bst_environ := BEnv (FEMPTY
+ |+ ("ProcState_C",BType_Imm Bit1, SOME(BVal_Imm (bool2b ms.PSTATE.C)))
+ |+ ("tmp_ProcState_C",BType_Imm Bit1, SOME(BVal_Imm (bool2b ms.PSTATE.C)))
+ |+ ("ProcState_N",BType_Imm Bit1, SOME(BVal_Imm (bool2b ms.PSTATE.N)))
+ |+ ("tmp_ProcState_N",BType_Imm Bit1, SOME(BVal_Imm (bool2b ms.PSTATE.N)))
+ |+ ("ProcState_V",BType_Imm Bit1, SOME(BVal_Imm (bool2b ms.PSTATE.V)))
+ |+ ("tmp_ProcState_V",BType_Imm Bit1, SOME(BVal_Imm (bool2b ms.PSTATE.V)))
+ |+ ("ProcState_Z",BType_Imm Bit1, SOME(BVal_Imm (bool2b ms.PSTATE.Z)))
+ |+ ("tmp_ProcState_Z",BType_Imm Bit1, SOME(BVal_Imm (bool2b ms.PSTATE.Z)))
+ |+ ("R0",BType_Imm Bit64, SOME(BVal_Imm (Imm64 (ms.REG 0w))))
+ |+ ("tmp_R0",BType_Imm Bit64, SOME(BVal_Imm (Imm64 (ms.REG 0w))))
+ |+ ("R1",BType_Imm Bit64, SOME(BVal_Imm (Imm64 (ms.REG 1w))))
+ |+ ("tmp_R1",BType_Imm Bit64, SOME(BVal_Imm (Imm64 (ms.REG 1w))))
+ |+ ("R2",BType_Imm Bit64, SOME(BVal_Imm (Imm64 (ms.REG 2w))))
+ |+ ("tmp_R2",BType_Imm Bit64, SOME(BVal_Imm (Imm64 (ms.REG 2w))))
+ |+ ("R3",BType_Imm Bit64, SOME(BVal_Imm (Imm64 (ms.REG 3w))))
+ |+ ("tmp_R3",BType_Imm Bit64, SOME(BVal_Imm (Imm64 (ms.REG 3w))))
+ |+ ("R4",BType_Imm Bit64, SOME(BVal_Imm (Imm64 (ms.REG 4w))))
+ |+ ("tmp_R4",BType_Imm Bit64, SOME(BVal_Imm (Imm64 (ms.REG 4w))))
+ |+ ("R5",BType_Imm Bit64, SOME(BVal_Imm (Imm64 (ms.REG 5w))))
+ |+ ("tmp_R5",BType_Imm Bit64, SOME(BVal_Imm (Imm64 (ms.REG 5w))))
+ |+ ("R6",BType_Imm Bit64, SOME(BVal_Imm (Imm64 (ms.REG 6w))))
+ |+ ("tmp_R6",BType_Imm Bit64, SOME(BVal_Imm (Imm64 (ms.REG 6w))))
+ |+ ("R7",BType_Imm Bit64, SOME(BVal_Imm (Imm64 (ms.REG 7w))))
+ |+ ("tmp_R7",BType_Imm Bit64, SOME(BVal_Imm (Imm64 (ms.REG 7w))))
+ |+ ("R8",BType_Imm Bit64, SOME(BVal_Imm (Imm64 (ms.REG 8w))))
+ |+ ("tmp_R8",BType_Imm Bit64, SOME(BVal_Imm (Imm64 (ms.REG 8w))))
+ |+ ("R9",BType_Imm Bit64, SOME(BVal_Imm (Imm64 (ms.REG 9w))))
+ |+ ("tmp_R9",BType_Imm Bit64, SOME(BVal_Imm (Imm64 (ms.REG 9w))))
+ |+ ("R10",BType_Imm Bit64, SOME(BVal_Imm (Imm64 (ms.REG 10w))))
+ |+ ("tmp_R10",BType_Imm Bit64, SOME(BVal_Imm (Imm64 (ms.REG 10w))))
+ |+ ("R11",BType_Imm Bit64, SOME(BVal_Imm (Imm64 (ms.REG 11w))))
+ |+ ("tmp_R11",BType_Imm Bit64, SOME(BVal_Imm (Imm64 (ms.REG 11w))))
+ |+ ("R12",BType_Imm Bit64, SOME(BVal_Imm (Imm64 (ms.REG 12w))))
+ |+ ("tmp_R12",BType_Imm Bit64, SOME(BVal_Imm (Imm64 (ms.REG 12w))))
+ |+ ("R13",BType_Imm Bit64, SOME(BVal_Imm (Imm64 (ms.REG 13w))))
+ |+ ("tmp_R13",BType_Imm Bit64, SOME(BVal_Imm (Imm64 (ms.REG 13w))))
+ |+ ("R14",BType_Imm Bit64, SOME(BVal_Imm (Imm64 (ms.REG 14w))))
+ |+ ("tmp_R14",BType_Imm Bit64, SOME(BVal_Imm (Imm64 (ms.REG 14w))))
+ |+ ("R15",BType_Imm Bit64, SOME(BVal_Imm (Imm64 (ms.REG 15w))))
+ |+ ("tmp_R15",BType_Imm Bit64, SOME(BVal_Imm (Imm64 (ms.REG 15w))))
+ |+ ("R16",BType_Imm Bit64, SOME(BVal_Imm (Imm64 (ms.REG 16w))))
+ |+ ("tmp_R16",BType_Imm Bit64, SOME(BVal_Imm (Imm64 (ms.REG 16w))))
+ |+ ("R17",BType_Imm Bit64, SOME(BVal_Imm (Imm64 (ms.REG 17w))))
+ |+ ("tmp_R17",BType_Imm Bit64, SOME(BVal_Imm (Imm64 (ms.REG 17w))))
+ |+ ("R18",BType_Imm Bit64, SOME(BVal_Imm (Imm64 (ms.REG 18w))))
+ |+ ("tmp_R18",BType_Imm Bit64, SOME(BVal_Imm (Imm64 (ms.REG 18w))))
+ |+ ("R19",BType_Imm Bit64, SOME(BVal_Imm (Imm64 (ms.REG 19w))))
+ |+ ("tmp_R19",BType_Imm Bit64, SOME(BVal_Imm (Imm64 (ms.REG 19w))))
+ |+ ("R20",BType_Imm Bit64, SOME(BVal_Imm (Imm64 (ms.REG 20w))))
+ |+ ("tmp_R20",BType_Imm Bit64, SOME(BVal_Imm (Imm64 (ms.REG 20w))))
+ |+ ("R21",BType_Imm Bit64, SOME(BVal_Imm (Imm64 (ms.REG 21w))))
+ |+ ("tmp_R21",BType_Imm Bit64, SOME(BVal_Imm (Imm64 (ms.REG 21w))))
+ |+ ("R22",BType_Imm Bit64, SOME(BVal_Imm (Imm64 (ms.REG 22w))))
+ |+ ("tmp_R22",BType_Imm Bit64, SOME(BVal_Imm (Imm64 (ms.REG 22w))))
+ |+ ("R23",BType_Imm Bit64, SOME(BVal_Imm (Imm64 (ms.REG 23w))))
+ |+ ("tmp_R23",BType_Imm Bit64, SOME(BVal_Imm (Imm64 (ms.REG 23w))))
+ |+ ("R24",BType_Imm Bit64, SOME(BVal_Imm (Imm64 (ms.REG 24w))))
+ |+ ("tmp_R24",BType_Imm Bit64, SOME(BVal_Imm (Imm64 (ms.REG 24w))))
+ |+ ("R25",BType_Imm Bit64, SOME(BVal_Imm (Imm64 (ms.REG 25w))))
+ |+ ("tmp_R25",BType_Imm Bit64, SOME(BVal_Imm (Imm64 (ms.REG 25w))))
+ |+ ("R26",BType_Imm Bit64, SOME(BVal_Imm (Imm64 (ms.REG 26w))))
+ |+ ("tmp_R26",BType_Imm Bit64, SOME(BVal_Imm (Imm64 (ms.REG 26w))))
+ |+ ("R27",BType_Imm Bit64, SOME(BVal_Imm (Imm64 (ms.REG 27w))))
+ |+ ("tmp_R27",BType_Imm Bit64, SOME(BVal_Imm (Imm64 (ms.REG 27w))))
+ |+ ("R28",BType_Imm Bit64, SOME(BVal_Imm (Imm64 (ms.REG 28w))))
+ |+ ("tmp_R28",BType_Imm Bit64, SOME(BVal_Imm (Imm64 (ms.REG 28w))))
+ |+ ("R29",BType_Imm Bit64, SOME(BVal_Imm (Imm64 (ms.REG 29w))))
+ |+ ("tmp_R29",BType_Imm Bit64, SOME(BVal_Imm (Imm64 (ms.REG 29w))))
+ |+ ("R30",BType_Imm Bit64, SOME(BVal_Imm (Imm64 (ms.REG 30w))))
+ |+ ("tmp_R30",BType_Imm Bit64, SOME(BVal_Imm (Imm64 (ms.REG 30w))))
+ |+ ("R31",BType_Imm Bit64, SOME(BVal_Imm (Imm64 (ms.REG 31w))))
+ |+ ("tmp_R31",BType_Imm Bit64, SOME(BVal_Imm (Imm64 (ms.REG 31w))))
+ |+ ("SP_EL0",BType_Imm Bit64, SOME(BVal_Imm (Imm64 (ms.SP_EL0))))
+ |+ ("tmp_SP_EL0",BType_Imm Bit64, SOME(BVal_Imm (Imm64 (ms.SP_EL0))))
+ |+ ("SP_EL1",BType_Imm Bit64, SOME(BVal_Imm (Imm64 (ms.SP_EL1))))
+ |+ ("tmp_SP_EL1",BType_Imm Bit64, SOME(BVal_Imm (Imm64 (ms.SP_EL1))))
+ |+ ("SP_EL2",BType_Imm Bit64, SOME(BVal_Imm (Imm64 (ms.SP_EL2))))
+ |+ ("tmp_SP_EL2",BType_Imm Bit64, SOME(BVal_Imm (Imm64 (ms.SP_EL2))))
+ |+ ("SP_EL3",BType_Imm Bit64, SOME(BVal_Imm (Imm64 (ms.SP_EL3))))
+ |+ ("tmp_SP_EL3",BType_Imm Bit64, SOME(BVal_Imm (Imm64 (ms.SP_EL3))))
+ |+ ("tmp_PC",BType_Imm Bit64, SOME(BVal_Imm (Imm64 (ms.PC))))
+ |+ ("MEM", (BType_Mem Bit64 Bit8), SOME(BVal_Mem Bit64 Bit8 (bir_mmap_w_w2n (bir_mf2mm ms.MEM))))
+ |+ ("tmp_MEM", (BType_Mem Bit64 Bit8), SOME(BVal_Mem Bit64 Bit8 (bir_mmap_w_w2n (bir_mf2mm ms.MEM))))
+ |+ ("tmp_COND",BType_Imm Bit1, SOME(BVal_Imm (Imm1 0w)))
+ );
+  bst_status := BST_Running|>
+`;
+
+
+val default_arm8_bir_state_satisfies_rel_thm = prove(``
+!ms .
+(arm8_bmr.bmr_extra ms) ==>
+   (bmr_rel arm8_bmr (default_arm8_bir_state ms) ms)
+``,
+REPEAT STRIP_TAC >>
+FULL_SIMP_TAC (std_ss) [default_arm8_bir_state_def,
+ bir_lifting_machinesTheory.arm8_bmr_rel_EVAL,
+ bir_envTheory.bir_env_var_is_declared_def,
+ bir_envTheory.bir_var_name_def] >>
+FULL_SIMP_TAC (srw_ss()) [
+              bir_envTheory.bir_env_read_UPDATE, bir_envTheory.bir_var_name_def,
+              bir_envTheory.bir_env_lookup_UPDATE,
+              bir_envTheory.bir_var_type_def, bir_envTheory.bir_env_lookup_type_def] >>
+FULL_SIMP_TAC (std_ss) [bir_lifting_machinesTheory.bmr_extra_ARM8] >>
+FULL_SIMP_TAC (srw_ss()) [bir_exp_liftingTheory.bir_load_w2n_mf_simp_thm] >>
+METIS_TAC []
+);
+
+
+val exist_bir_of_arm8_thm = prove(``
+!ms vars .
+(arm8_wf_varset vars) ==>
+(arm8_bmr.bmr_extra ms) ==>
+? bs .((bmr_rel arm8_bmr bs ms) /\ (bs.bst_status = BST_Running) /\ (bir_env_vars_are_initialised bs.bst_environ vars))
+``,
+REPEAT STRIP_TAC >> 
+EXISTS_TAC ``default_arm8_bir_state ms`` >>
+ASSUME_TAC (SPEC ``ms:arm8_state`` default_arm8_bir_state_satisfies_rel_thm) >>
+FULL_SIMP_TAC (std_ss) [] >>
+STRIP_TAC >-  EVAL_TAC >>
+PAT_X_ASSUM ``arm8_wf_varset vars`` (fn thm=> REWRITE_TAC [SIMP_RULE std_ss [arm8_wf_varset_def] thm]) >>
+FULL_SIMP_TAC (std_ss) [bir_envTheory.bir_env_vars_are_initialised_INSERT] >>
+REPEAT STRIP_TAC >>
+FULL_SIMP_TAC (std_ss) [bir_envTheory.bir_env_var_is_initialised_def] >>
+FULL_SIMP_TAC (std_ss) [bir_envTheory.bir_var_name_def, default_arm8_bir_state_def, bir_envTheory.bir_env_lookup_UPDATE] >>
+EVAL_TAC>>
+FULL_SIMP_TAC std_ss [bir_valuesTheory.bir_val_t_11, bir_immTheory.type_of_bir_imm_def, bir_valuesTheory.type_of_bir_val_EQ_ELIMS]
+);
+
+val set_of_address_in_all_address_labels_thm = prove (``
+!l adds.
+(l ∈ {BL_Address (Imm64 ml') | ml' ∈ adds}) ==>
+(l ∈ {l | IS_BL_Address l})
+``,
+REPEAT STRIP_TAC >>
+FULL_SIMP_TAC (std_ss) [pred_setTheory.GSPECIFICATION, bir_program_labelsTheory.IS_BL_Address_def]
+);
+
+(*
+ bir_programTheory.bir_programcounter_t_component_equality
+ *)
+ 
+
 (* Code specific for the example *)
 
 
@@ -181,7 +420,7 @@ FULL_SIMP_TAC (std_ss) [b_sqrt_I_def, bir_expTheory.bir_eval_exp_def] >>
   [(UNDISCH o (SPECL [``bs:bir_state_t``, ``ms:arm8_state``])) bload_64_to_arm8_load_64_thm] @
   [bir_bool_expTheory.BVal_Imm_bool2b_EQ_TF_REWRS, bir_valuesTheory.BType_Bool_def ])) >>
 FULL_SIMP_TAC (std_ss) [arm8_sqrt_I_def] >>
-FULL_SIMP_TAC (std_ss) [bir_immTheory.bool2w_11, bool2w_and, bir_bool_expTheory.bir_val_true_def, imm_eq_to_val_eq, bir_bool_expTheory.bool2w_ELIMS] >>
+FULL_SIMP_TAC (std_ss) [bir_immTheory.bool2w_11, bool2w_and, bir_bool_expTheory.bir_val_true_def, imm_eq_to_val_eq, bir_bool_expTheory.bool2w_ELIMS] 
 );
 
 
